start to have some mudularity

tttree.dfy
@@ -1,341 +1,511 @@
-type Key = int
+include "total_order.dfy"
+include "map_utils.dfy"
+include "mathematics.dfy"
 
-predicate method key_lt(a: Key, b: Key)
-	ensures key_lt(a, b) ==> a != b;
-{
-	a < b
-}
-
-datatype Node<Value> =
-	Leaf(key: Key, value: Value) |
-	TwoNode(left: Node, pivot: Key,
-	        right: Node) |
-	ThreeNode(left: Node, pivota: Key,
-	          middle: Node, pivotb: Key,
-						right: Node)
-
-function merge_maps<U,T>(mapa: map<U,T>, mapb: map<U,T>) : map<U,T>
-	ensures merge_maps(mapa, mapb).Keys == mapa.Keys + mapb.Keys;
-	ensures forall k :: k in merge_maps(mapa, mapb).Keys && k !in mapb.Keys ==>
-		merge_maps(mapa, mapb)[k] == mapa[k];
-	ensures forall k :: k in merge_maps(mapa, mapb).Keys && k !in mapa.Keys ==>
-		merge_maps(mapa, mapb)[k] == mapb[k];
-	ensures forall k :: k in merge_maps(mapa, mapb).Keys && k in mapa.Keys * mapb.Keys ==>
-		merge_maps(mapa, mapb)[k] == mapa[k] || merge_maps(mapa, mapb)[k] == mapb[k];
-{
-	map x : U | (x in mapa.Keys + mapb.Keys) :: if x in mapa then mapa[x] else mapb[x]
-}
-
-function SubtreeAllKeys(tree: Node) : set<Key>
-{
-	match tree {
-		case Leaf(key, value) => {key}
-		case TwoNode(left, pivot, right) => SubtreeAllKeys(left) + {pivot} + SubtreeAllKeys(right)
-		case ThreeNode(left, pivota, middle, pivotb, right) =>
-			SubtreeAllKeys(left) + {pivota} + SubtreeAllKeys(middle) + {pivotb} + SubtreeAllKeys(right)
-	}
-}
-
-function SubtreeContents<Value>(tree: Node<Value>) : map<int, Value>
-	ensures SubtreeContents(tree).Keys <= SubtreeAllKeys(tree);
-{
-	if tree.Leaf? then
-		var r := map[tree.key := tree.value];
-		assert tree.key in r; // observe that r is not friggin empty
-		r
-	else if tree.TwoNode?
-    then merge_maps(SubtreeContents(tree.left), SubtreeContents(tree.right))
-	else 
-		merge_maps(
-		merge_maps(SubtreeContents(tree.left), SubtreeContents(tree.middle)),
-		SubtreeContents(tree.right))
-}
-
-predicate ContentsAreLessThan(tree: Node, pivot: int) {
-	forall lv :: lv in SubtreeAllKeys(tree) ==> key_lt(lv, pivot)
-}
-
-predicate ContentsAreGreaterEqualThan(pivot: int, tree: Node) {
-	forall lv :: lv in SubtreeAllKeys(tree) ==> !key_lt(lv, pivot)
-}
-
-predicate OrderedTree(tree: Node) {
-  if tree.Leaf?
-		then true
-	else if tree.TwoNode?
-    then
-		ContentsAreLessThan(tree.left, tree.pivot) &&
-		ContentsAreGreaterEqualThan(tree.pivot, tree.right) &&
-		OrderedTree(tree.left) &&
-		OrderedTree(tree.right)
-	else
-		key_lt(tree.pivota, tree.pivotb) &&
-		ContentsAreLessThan(tree.left, tree.pivota) &&
-		ContentsAreGreaterEqualThan(tree.pivota, tree.middle) &&
-		ContentsAreLessThan(tree.middle, tree.pivotb) &&
-		ContentsAreGreaterEqualThan(tree.pivotb, tree.right) &&
-		OrderedTree(tree.left) &&
-		OrderedTree(tree.middle) &&
-		OrderedTree(tree.right)
-}
-
-function min(a: int, b: int) : int
-{
-	if a < b
-		then a
-	else
-		b
-}
-
-function max(a: int, b: int) : int
-{
-	if a < b
-		then b
-	else
-		a
-}
-
-function minHeight(tree: Node) : int
-{
-	if tree.Leaf?
-		then 0
-	else if tree.TwoNode?
-		then 1 + min(minHeight(tree.left), minHeight(tree.right))
-	else 
-		1 + min(minHeight(tree.left), min(minHeight(tree.middle), minHeight(tree.right)))
-}
-
-function maxHeight(tree: Node) : int
-{
-	if tree.Leaf?
-		then 0
-	else if tree.TwoNode?
-		then 1 + max(maxHeight(tree.left), maxHeight(tree.right))
-	else
-		1 + max(maxHeight(tree.left), max(maxHeight(tree.middle), maxHeight(tree.right)))
-}
-
-predicate balanced(tree: Node) {
-	minHeight(tree) == maxHeight(tree)
-}
-
-predicate TTSubtree(tree: Node) {
-
-	if tree.Leaf?
-		then OrderedTree(tree) &&
-		balanced(tree)
-	else if tree.TwoNode?
-		then OrderedTree(tree) &&
-		balanced(tree) &&
-		TTSubtree(tree.left) &&
-		TTSubtree(tree.right)
-	else
-		OrderedTree(tree) &&
-		balanced(tree) &&
-		TTSubtree(tree.left) &&
-		TTSubtree(tree.middle) &&
-		TTSubtree(tree.right)
-}
-
-function Height(tree: Node) : int
-	requires(balanced(tree));
-{
-	minHeight(tree)
-}
-
-function method mkTwoNode(t1: Node, pivot: Key, t2: Node) : Node
-	requires TTSubtree(t1);
-	requires TTSubtree(t2);
-	requires Height(t1) == Height(t2);
-	requires ContentsAreLessThan(t1, pivot);
-	requires ContentsAreGreaterEqualThan(pivot, t2);
-	ensures TTSubtree(mkTwoNode(t1, pivot, t2));
-	ensures Height(mkTwoNode(t1, pivot, t2)) == Height(t1) + 1;
-{
-	TwoNode(t1, pivot, t2)
-}
-
-function method mkThreeNode(t1: Node, pivota: Key, t2: Node, pivotb: Key, t3: Node) : Node
-	requires TTSubtree(t1);
-	requires TTSubtree(t2);
-	requires TTSubtree(t3);
-	requires Height(t1) == Height(t2) == Height(t3);
-	requires key_lt(pivota, pivotb);
-	requires ContentsAreLessThan(t1, pivota);
-	requires ContentsAreGreaterEqualThan(pivota, t2);
-	requires ContentsAreLessThan(t2, pivotb);
-	requires ContentsAreGreaterEqualThan(pivotb, t3);
-	ensures TTSubtree(mkThreeNode(t1, pivota, t2, pivotb, t3));
-	ensures Height(mkThreeNode(t1, pivota, t2, pivotb, t3)) == Height(t1) + 1;
-{
-	ThreeNode(t1, pivota, t2, pivotb, t3)
-}
-
-datatype QueryResult<Value> = KeyDoesNotExist | ValueForKey(value: Value)
-
-function method QuerySubtree<Value>(tree: Node<Value>, key: Key) : QueryResult<Value>
-    requires OrderedTree(tree);
-    ensures QuerySubtree(tree, key) == KeyDoesNotExist <==>
-			(key !in SubtreeContents(tree));
-		ensures QuerySubtree(tree, key).ValueForKey? <==>
-			(key in SubtreeContents(tree) && SubtreeContents(tree)[key] == QuerySubtree(tree, key).value);
-{
-	if tree.Leaf? && tree.key == key then
-		ValueForKey(tree.value)
-	else if tree.Leaf? && tree.key != key then
-		KeyDoesNotExist
-	else if tree.TwoNode? && key_lt(key, tree.pivot) then
-		QuerySubtree(tree.left, key)
-	else if tree.TwoNode? && !key_lt(key, tree.pivot) then
-		QuerySubtree(tree.right, key)
-	else if tree.ThreeNode? && key_lt(key, tree.pivota) then
-		QuerySubtree(tree.left, key)
-	else if tree.ThreeNode? && key_lt(key, tree.pivotb) then
-		QuerySubtree(tree.middle, key)
-	else
-		QuerySubtree(tree.right, key)
-}
-
-datatype InsertionResult<Value> = InsertionResult(tree: Node<Value>, split: bool)
+abstract module TwoThreeTree {
+	import Keyspace : Totally_Ordered_Type
+	import Maps = Map_Utils
+	import Math = Mathematics
 	
-method InsertIntoSubtree<Value>(tree: Node<Value>, key: Key, value: Value)
-	returns (result: InsertionResult<Value>)
-	requires TTSubtree(tree);
-	ensures TTSubtree(result.tree);
-	ensures SubtreeAllKeys(result.tree) == SubtreeAllKeys(tree) + {key};
-	ensures SubtreeContents(result.tree) == SubtreeContents(tree)[key := value];
-	ensures result.split ==> result.tree.TwoNode?;
-	ensures result.split ==> result.tree.pivot in SubtreeAllKeys(tree) + {key};
-	ensures result.split ==> Height(result.tree) == Height(tree) + 1;
-	ensures !result.split ==> Height(result.tree) == Height(tree);
-{
-	if tree.Leaf? {
-		if tree.key == key {
-			result := InsertionResult(Leaf(key, value), false);
-		} else if key_lt(tree.key, key) {
-			var newright := Leaf(key, value);
-			var newtree := mkTwoNode(tree, key, newright);
-			assert(Height(newright) == Height(tree));
-			assert(Height(newtree) == Height(tree) + 1);
-			result := InsertionResult(newtree, true);
-		} else {
-			var newleft := Leaf(key, value);
-			var newtree := mkTwoNode(newleft, tree.key, tree);
-			assert(Height(newleft) == Height(tree));
-			assert(Height(newtree) == Height(tree) + 1);
-			result := InsertionResult(newtree, true);
-		}
-	} else if tree.TwoNode? {
-		if key_lt(key, tree.pivot) {
-			var subresult := InsertIntoSubtree(tree.left, key, value);
-			if !subresult.split {
-				result := InsertionResult(mkTwoNode(subresult.tree, tree.pivot, tree.right), false);
-			} else {
-				assert SubtreeAllKeys(subresult.tree.right) != {};
-				assert key_lt(subresult.tree.pivot, tree.pivot);
-				result := InsertionResult(mkThreeNode(subresult.tree.left, subresult.tree.pivot,
-					                                   subresult.tree.right, tree.pivot,
-																					   tree.right), false);
-			}
-		} else {
-			var subresult := InsertIntoSubtree(tree.right, key, value);
-			if !subresult.split {
-				result := InsertionResult(mkTwoNode(tree.left, tree.pivot, subresult.tree), false);
-			} else {
-				result := InsertionResult(mkThreeNode(tree.left, tree.pivot,
-			                		                   subresult.tree.left, subresult.tree.pivot,
-																						 subresult.tree.right), false);
-			}
-		}
-	} else if tree.ThreeNode? {
-		if key_lt(key, tree.pivota) {
-			var subresult := InsertIntoSubtree(tree.left, key, value);
-			if !subresult.split {
-				result := InsertionResult(mkThreeNode(subresult.tree, tree.pivota,
-					                                   tree.middle, tree.pivotb,
-																						 tree.right), false);
-			} else {
-				var newright := mkTwoNode(tree.middle, tree.pivotb, tree.right);
-				assert(Height(newright) == Height(tree));
-				var newtree := mkTwoNode(subresult.tree, tree.pivota, newright);
-				assert(Height(newtree) == Height(tree) + 1);
-				result := InsertionResult(newtree, true);
-			}
-		} else if key_lt(key, tree.pivotb) {
-			var subresult := InsertIntoSubtree(tree.middle, key, value);
-			if !subresult.split {
-				result := InsertionResult(mkThreeNode(tree.left, tree.pivota,
-					                                   subresult.tree, tree.pivotb,
-																						 tree.right), false);
-			} else {
-				var newleft := mkTwoNode(tree.left, tree.pivota, subresult.tree.left);
-				var newright := mkTwoNode(subresult.tree.right, tree.pivotb, tree.right);
-				var newtree := mkTwoNode(newleft, subresult.tree.pivot, newright);
-				assert(Height(newleft) == Height(tree));
-				assert(Height(newright) == Height(tree));
-				assert(Height(newtree) == Height(tree) + 1);
-				result := InsertionResult(newtree, true);
-			}
-		} else {
-			var subresult := InsertIntoSubtree(tree.right, key, value);
-			if !subresult.split {
-				result := InsertionResult(mkThreeNode(tree.left, tree.pivota,
-					                                   tree.middle, tree.pivotb,
-																						 subresult.tree), false);
-			} else {
-				var newleft := TwoNode(tree.left, tree.pivota, tree.middle);
-				var newtree := TwoNode(newleft, tree.pivotb, subresult.tree);
-				assert(Height(newleft) == Height(tree));
-				assert(Height(newtree) == Height(tree) + 1);
-				result := InsertionResult(newtree, true);
-			}
-		}
-	} 
-}
+	datatype Node<Value> =
+		Leaf(key: Keyspace.Element, value: Value) |
+		TwoNode(left: Node, pivot: Keyspace.Element,
+	  right: Node) |
+		ThreeNode(left: Node, pivota: Keyspace.Element,
+	  middle: Node, pivotb: Keyspace.Element,
+		right: Node)
 
-datatype Tree<Value> = EmptyTree | NonEmptyTree(root: Node<Value>)
+		function SubtreeAllKeys(tree: Node) : set<Keyspace.Element>
+			ensures SubtreeAllKeys(tree) != {};
+		{
+			match tree {
+				case Leaf(key, value) => {key}
+				case TwoNode(left, pivot, right) => SubtreeAllKeys(left) + {pivot} + SubtreeAllKeys(right)
+				case ThreeNode(left, pivota, middle, pivotb, right) =>
+					SubtreeAllKeys(left) + {pivota} + SubtreeAllKeys(middle) + {pivotb} + SubtreeAllKeys(right)
+			}
+		}
+
+		predicate ContentsAreLessThan(tree: Node, pivot: Keyspace.Element) {
+			forall lv :: lv in SubtreeAllKeys(tree) ==> Keyspace.lt(lv, pivot)
+		}
+
+		predicate ContentsAreGreaterEqualThan(pivot: Keyspace.Element, tree: Node) {
+			forall lv :: lv in SubtreeAllKeys(tree) ==> !Keyspace.lt(lv, pivot)
+		}
+
+		predicate TreeIsOrdered(tree: Node) {
+			if tree.Leaf?
+				then true
+			else if tree.TwoNode?
+				then
+				ContentsAreLessThan(tree.left, tree.pivot) &&
+				ContentsAreGreaterEqualThan(tree.pivot, tree.right) &&
+				TreeIsOrdered(tree.left) &&
+				TreeIsOrdered(tree.right)
+			else
+				Keyspace.lt(tree.pivota, tree.pivotb) &&
+				ContentsAreLessThan(tree.left, tree.pivota) &&
+				ContentsAreGreaterEqualThan(tree.pivota, tree.middle) &&
+				ContentsAreLessThan(tree.middle, tree.pivotb) &&
+				ContentsAreGreaterEqualThan(tree.pivotb, tree.right) &&
+				TreeIsOrdered(tree.left) &&
+				TreeIsOrdered(tree.middle) &&
+				TreeIsOrdered(tree.right)
+		}
+
+ 		function SubtreeContents<Value>(tree: Node<Value>) : map<Keyspace.Element, Value>
+			requires TreeIsOrdered(tree);
+			ensures SubtreeContents(tree).Keys <= SubtreeAllKeys(tree);
+			ensures SubtreeContents(tree) != map[];
+		{
+			if tree.Leaf? then
+				var r := map[tree.key := tree.value];
+				assert tree.key in r; // observe that r is not friggin empty
+				r
+			else if tree.TwoNode? then
+				Maps.disjoint_union(SubtreeContents(tree.left), SubtreeContents(tree.right))
+			else
+				var lmentries := Maps.disjoint_union(SubtreeContents(tree.left), SubtreeContents(tree.middle));
+				Maps.disjoint_union(lmentries, SubtreeContents(tree.right))
+		}
+
+		datatype QueryResult<Value> = KeyDoesNotExist | ValueForKey(value: Value)
+
+		function method QuerySubtree<Value>(tree: Node<Value>, key: Keyspace.Element) : QueryResult<Value>
+			requires TreeIsOrdered(tree);
+			ensures QuerySubtree(tree, key) == KeyDoesNotExist <==>
+				(key !in SubtreeContents(tree));
+				ensures QuerySubtree(tree, key).ValueForKey? <==>
+					(key in SubtreeContents(tree) && SubtreeContents(tree)[key] == QuerySubtree(tree, key).value);
+		{
+			if tree.Leaf? && tree.key == key then
+				ValueForKey(tree.value)
+			else if tree.Leaf? && tree.key != key then
+				KeyDoesNotExist
+			else if tree.TwoNode? && Keyspace.lt(key, tree.pivot) then
+				QuerySubtree(tree.left, key)
+			else if tree.TwoNode? && !Keyspace.lt(key, tree.pivot) then
+				QuerySubtree(tree.right, key)
+			else if tree.ThreeNode? && Keyspace.lt(key, tree.pivota) then
+				QuerySubtree(tree.left, key)
+			else if tree.ThreeNode? && Keyspace.lt(key, tree.pivotb) then
+				QuerySubtree(tree.middle, key)
+			else
+				QuerySubtree(tree.right, key)
+		}
+
+		function minHeight(tree: Node) : int
+		{
+			if tree.Leaf?
+				then 0
+			else if tree.TwoNode?
+				then 1 + Math.min(minHeight(tree.left), minHeight(tree.right))
+			else 
+				1 + Math.min(minHeight(tree.left), Math.min(minHeight(tree.middle), minHeight(tree.right)))
+		}
+
+		function maxHeight(tree: Node) : int
+		{
+			if tree.Leaf?
+				then 0
+			else if tree.TwoNode?
+				then 1 + Math.max(maxHeight(tree.left), maxHeight(tree.right))
+			else
+				1 + Math.max(maxHeight(tree.left), Math.max(maxHeight(tree.middle), maxHeight(tree.right)))
+		}
+
+		predicate balanced(tree: Node) {
+			minHeight(tree) == maxHeight(tree)
+		}
+
+		predicate TTSubtree(tree: Node) {
+
+			if tree.Leaf?
+				then TreeIsOrdered(tree) &&
+				balanced(tree)
+			else if tree.TwoNode?
+				then TreeIsOrdered(tree) &&
+				balanced(tree) &&
+				TTSubtree(tree.left) &&
+				TTSubtree(tree.right)
+			else
+				TreeIsOrdered(tree) &&
+				balanced(tree) &&
+				TTSubtree(tree.left) &&
+				TTSubtree(tree.middle) &&
+				TTSubtree(tree.right)
+		}
+
+		function Height(tree: Node) : int
+			requires(balanced(tree));
+		{
+			minHeight(tree)
+		}
+
+		function method mkTwoNode(t1: Node, pivot: Keyspace.Element, t2: Node) : Node
+			requires TTSubtree(t1);
+			requires TTSubtree(t2);
+			requires Height(t1) == Height(t2);
+			requires ContentsAreLessThan(t1, pivot);
+			requires ContentsAreGreaterEqualThan(pivot, t2);
+			ensures TTSubtree(mkTwoNode(t1, pivot, t2));
+			ensures SubtreeAllKeys(mkTwoNode(t1, pivot, t2)) == SubtreeAllKeys(t1) + { pivot } + SubtreeAllKeys(t2);
+			ensures SubtreeContents(mkTwoNode(t1, pivot, t2)) ==
+				Maps.disjoint_union(SubtreeContents(t1), SubtreeContents(t2));
+			ensures Height(mkTwoNode(t1, pivot, t2)) == Height(t1) + 1;
+		{
+			TwoNode(t1, pivot, t2)
+		}
+
+		function method mkThreeNode(t1: Node, pivota: Keyspace.Element,
+			                          t2: Node, pivotb: Keyspace.Element, 
+																t3: Node) : Node
+      requires TTSubtree(t1);
+			requires TTSubtree(t2);
+			requires TTSubtree(t3);
+			requires Height(t1) == Height(t2) == Height(t3);
+			requires Keyspace.lt(pivota, pivotb);
+			requires ContentsAreLessThan(t1, pivota);
+			requires ContentsAreGreaterEqualThan(pivota, t2);
+			requires ContentsAreLessThan(t2, pivotb);
+			requires ContentsAreGreaterEqualThan(pivotb, t3);
+			ensures TTSubtree(mkThreeNode(t1, pivota, t2, pivotb, t3));
+			ensures SubtreeAllKeys(mkThreeNode(t1, pivota, t2, pivotb, t3)) ==
+				SubtreeAllKeys(t1) + { pivota } + SubtreeAllKeys(t2) + { pivotb } + SubtreeAllKeys(t3);
+			ensures SubtreeContents(mkThreeNode(t1, pivota, t2, pivotb, t3)) ==
+				Maps.disjoint_union(Maps.disjoint_union(SubtreeContents(t1), SubtreeContents(t2)), 
+				                   SubtreeContents(t3));
+			ensures Height(mkThreeNode(t1, pivota, t2, pivotb, t3)) == Height(t1) + 1;
+		{
+			ThreeNode(t1, pivota, t2, pivotb, t3)
+		}
+
+		datatype InsertionResult<Value> = InsertionResult(tree: Node<Value>, split: bool)
+
+		predicate ValidInsertionResult<Value>(result: InsertionResult<Value>, tree: Node<Value>,
+			key: Keyspace.Element, value: Value)
+			requires TTSubtree(tree);
+		{
+			 TTSubtree(result.tree) &&
+				(SubtreeAllKeys(result.tree) == SubtreeAllKeys(tree) + {key}) &&
+				(SubtreeContents(result.tree) == SubtreeContents(tree)[key := value]) &&
+				(result.split ==> result.tree.TwoNode?) &&
+				(result.split ==> result.tree.pivot in SubtreeAllKeys(tree) + {key}) &&
+				(result.split ==> Height(result.tree) == Height(tree) + 1) &&
+				(!result.split ==> Height(result.tree) == Height(tree))
+		}
+
+		method InsertIntoLeaf<Value>(tree: Node<Value>, key: Keyspace.Element, value: Value)
+			returns (result: InsertionResult<Value>)
+			requires TTSubtree(tree);
+			requires tree.Leaf?;
+			ensures ValidInsertionResult(result, tree, key, value);
+		{
+			if tree.key == key {
+				result := InsertionResult(Leaf(key, value), false);
+			} else if Keyspace.lt(tree.key, key) {
+				var newright := Leaf(key, value);
+				var newtree := mkTwoNode(tree, key, newright);
+				assert(Height(newright) == Height(tree));
+				assert(Height(newtree) == Height(tree) + 1);
+				result := InsertionResult(newtree, true);
+			} else {
+				var newleft := Leaf(key, value);
+				var newtree := mkTwoNode(newleft, tree.key, tree);
+				assert(Height(newleft) == Height(tree));
+				assert(Height(newtree) == Height(tree) + 1);
+				result := InsertionResult(newtree, true);
+			}
+		}
+
+		// method InsertIntoTwoNodeLeft<Value>(tree: Node<Value>, key: Keyspace.Element, value: Value)
+		// 	returns (result: InsertionResult<Value>)
+		// 	requires TTSubtree(tree);
+		// 	requires tree.TwoNode?;
+		// 	requires Keyspace.lt(key, tree.pivot);
+		// 	ensures ValidInsertionResult(result, tree, key, value);
+		// 	decreases tree, 0;
+		// {
+		// 	var subresult := InsertIntoSubtree(tree.left, key, value);
+		// 	if !subresult.split {
+		// 		result := InsertionResult(mkTwoNode(subresult.tree, tree.pivot, tree.right), false);
+		// 	} else {
+		// 		result := InsertionResult(mkThreeNode(subresult.tree.left, subresult.tree.pivot,
+		// 			subresult.tree.right, tree.pivot,
+		// 			tree.right), false);
+		// 	}
+		// }
+
+		// method InsertIntoTwoNodeRight<Value>(tree: Node<Value>, key: Keyspace.Element, value: Value)
+		// 	returns (result: InsertionResult<Value>)
+		// 	requires TTSubtree(tree);
+		// 	requires tree.TwoNode?;
+		// 	requires key == tree.pivot || Keyspace.lt(tree.pivot, key);
+		// 	ensures ValidInsertionResult(result, tree, key, value);
+		// 	decreases tree, 0;
+		// {
+		// 	var subresult := InsertIntoSubtree(tree.right, key, value);
+		// 	if !subresult.split {
+		// 		result := InsertionResult(mkTwoNode(tree.left, tree.pivot, subresult.tree), false);
+		// 	} else {
+		// 		result := InsertionResult(mkThreeNode(tree.left, tree.pivot,
+		// 	    subresult.tree.left, subresult.tree.pivot,
+		// 			subresult.tree.right), false);
+		// 	}
+		// }
+
+		// method InsertIntoTwoNode<Value>(tree: Node<Value>, key: Keyspace.Element, value: Value)
+		// 	returns (result: InsertionResult<Value>)
+		// 	requires TTSubtree(tree);
+		// 	requires tree.TwoNode?;
+		// 	requires key == tree.pivot || Keyspace.lt(tree.pivot, key);
+		// 	ensures ValidInsertionResult(result, tree, key, value);
+		// 	decreases tree, 1;
+		// {
+		// 	if Keyspace.lt(key, tree.pivot) {
+		// 		result := InsertIntoTwoNodeLeft(tree, key, value);
+		// 	} else {
+		// 		result := InsertIntoTwoNodeRight(tree, key, value);
+		// 	}
+		// }
 		
-predicate TTTree<Value>(tree: Tree<Value>) {
-	tree.EmptyTree? || TTSubtree(tree.root)
-}
+		// method InsertIntoThreeNodeLeft<Value>(tree: Node<Value>, key: Keyspace.Element, value: Value)
+		// 	returns (result: InsertionResult<Value>)
+		// 	requires TTSubtree(tree);
+		// 	requires tree.ThreeNode?;
+		// 	requires Keyspace.lt(key, tree.pivota);
+		// 	ensures ValidInsertionResult(result, tree, key, value);
+		// 	decreases tree, 0;
+		// {
+		// 	var subresult := InsertIntoSubtree(tree.left, key, value);
+		// 	if !subresult.split {
+		// 		result := InsertionResult(mkThreeNode(subresult.tree, tree.pivota,
+		// 			tree.middle, tree.pivotb,
+		// 			tree.right), false);
+		// 	} else {
+		// 		var newright := mkTwoNode(tree.middle, tree.pivotb, tree.right);
+		// 		assert(Height(newright) == Height(tree));
+		// 		var newtree := mkTwoNode(subresult.tree, tree.pivota, newright);
+		// 		assert(Height(newtree) == Height(tree) + 1);
+		// 		result := InsertionResult(newtree, true);
+		// 	}
+		// }
 
-function Contents<Value>(tree: Tree<Value>) : map<int, Value>
-{
-	if tree.EmptyTree?
-		then map[]
-	else
-		SubtreeContents(tree.root)
-}
+		// method InsertIntoThreeNodeMiddle<Value>(tree: Node<Value>, key: Keyspace.Element, value: Value)
+		// 	returns (result: InsertionResult<Value>)
+		// 	requires TTSubtree(tree);
+		// 	requires tree.ThreeNode?;
+		// 	requires (tree.pivota == key || Keyspace.lt(tree.pivota, key));
+		// 	requires Keyspace.lt(key, tree.pivotb);
+		// 	ensures ValidInsertionResult(result, tree, key, value);
+		// 	decreases tree, 0;
+		// {
+		// 	var subresult := InsertIntoSubtree(tree.middle, key, value);
+		// 	if !subresult.split {
+		// 		result := InsertionResult(mkThreeNode(tree.left, tree.pivota,
+		// 			subresult.tree, tree.pivotb,
+		// 			tree.right), false);
+		// 	} else {
+		// 		var newleft := mkTwoNode(tree.left, tree.pivota, subresult.tree.left);
+		// 		var newright := mkTwoNode(subresult.tree.right, tree.pivotb, tree.right);
+		// 		var newtree := mkTwoNode(newleft, subresult.tree.pivot, newright);
+		// 		assert(Height(newleft) == Height(tree));
+		// 		assert(Height(newright) == Height(tree));
+		// 		assert(Height(newtree) == Height(tree) + 1);
+		// 		result := InsertionResult(newtree, true);
+		// 	}
+		// }
 
-function method Query<Value>(tree: Tree<Value>, key: int) : QueryResult<Value>
-	requires(TTTree(tree));
-  ensures Query(tree, key) == KeyDoesNotExist <==>
-		(key !in Contents(tree));
-  ensures Query(tree, key).ValueForKey? <==>
-		(key in Contents(tree) && Contents(tree)[key] == Query(tree, key).value);
-{
-	if tree.EmptyTree? then
-		KeyDoesNotExist
-	else
-		QuerySubtree(tree.root, key)
-}
+		// method InsertIntoThreeNodeRight<Value>(tree: Node<Value>, key: Keyspace.Element, value: Value)
+		// 	returns (result: InsertionResult<Value>)
+		// 	requires TTSubtree(tree);
+		// 	requires tree.ThreeNode?;
+		// 	requires tree.pivotb == key || Keyspace.lt(tree.pivotb, key);
+		// 	ensures ValidInsertionResult(result, tree, key, value);
+		// 	decreases tree, 0;
+		// {
+		// 	var subresult := InsertIntoSubtree(tree.right, key, value);
+		// 	if !subresult.split {
+		// 		result := InsertionResult(mkThreeNode(tree.left, tree.pivota,
+		// 			tree.middle, tree.pivotb,
+		// 			subresult.tree), false);
+		// 	} else {
+		// 		var newleft := TwoNode(tree.left, tree.pivota, tree.middle);
+		// 		var newtree := TwoNode(newleft, tree.pivotb, subresult.tree);
+		// 		assert(Height(newleft) == Height(tree));
+		// 		assert(Height(newtree) == Height(tree) + 1);
+		// 		result := InsertionResult(newtree, true);
+		// 	}
+		// }
 
-method Insert<Value>(tree: Tree<Value>, key: int, value: Value) returns (newtree: Tree<Value>)
-	requires TTTree(tree);
-	ensures TTTree(newtree);
-	ensures Contents(newtree) == Contents(tree)[key := value];
-	ensures newtree.NonEmptyTree?;
-{
-	if tree.EmptyTree? {
-		newtree := NonEmptyTree(Leaf(key, value));
-	} else {
-		var result := InsertIntoSubtree(tree.root, key, value);
-		newtree := NonEmptyTree(result.tree);
-	}
-}
+		// method InsertIntoThreeNode<Value>(tree: Node<Value>, key: Keyspace.Element, value: Value)
+		// 	returns (result: InsertionResult<Value>)
+		// 	requires TTSubtree(tree);
+		// 	requires tree.ThreeNode?;
+		// 	ensures ValidInsertionResult(result, tree, key, value);
+		// 	decreases tree, 1;
+		// {
+		// 	if Keyspace.lt(key, tree.pivota) {
+		// 		result := InsertIntoThreeNodeLeft(tree, key, value);
+		// 	} else if Keyspace.lt(key, tree.pivotb) {
+		// 		result := InsertIntoThreeNodeMiddle(tree, key, value);
+		// 	} else {
+		// 		result := InsertIntoThreeNodeRight(tree, key, value);
+		// 	}
+		// }
+		
+		method InsertIntoSubtree<Value>(tree: Node<Value>, key: Keyspace.Element, value: Value)
+			returns (result: InsertionResult<Value>)
+			requires TTSubtree(tree);
+			ensures ValidInsertionResult(result, tree, key, value);
+			decreases tree, 3;
+		{
+			// if tree.Leaf? {
+			// 	result := InsertIntoLeaf(tree, key, value);
+			// } else if tree.TwoNode? {
+			// 	result := InsertIntoTwoNode(tree, key, value);
+			// } else {
+			// 	result := InsertIntoThreeNode(tree, key, value);
+			// }
+		}
+		
+		// method InsertIntoSubtree<Value>(tree: Node<Value>, key: Keyspace.Element, value: Value)
+		// 	returns (result: InsertionResult<Value>)
+		// 	requires TTSubtree(tree);
+		// 	ensures TTSubtree(result.tree);
+		// 	ensures SubtreeAllKeys(result.tree) == SubtreeAllKeys(tree) + {key};
+		// 	ensures SubtreeContents(result.tree) == SubtreeContents(tree)[key := value];
+		// 	ensures result.split ==> result.tree.TwoNode?;
+		// 	ensures result.split ==> result.tree.pivot in SubtreeAllKeys(tree) + {key};
+		// 	ensures result.split ==> Height(result.tree) == Height(tree) + 1;
+		// 	ensures !result.split ==> Height(result.tree) == Height(tree);
+		// {
+		// 	if tree.Leaf? {
+		// 		if tree.key == key {
+		// 			result := InsertionResult(Leaf(key, value), false);
+		// 		} else if Keyspace.lt(tree.key, key) {
+		// 			var newright := Leaf(key, value);
+		// 			var newtree := mkTwoNode(tree, key, newright);
+		// 			assert(Height(newright) == Height(tree));
+		// 			assert(Height(newtree) == Height(tree) + 1);
+		// 			result := InsertionResult(newtree, true);
+		// 		} else {
+		// 			var newleft := Leaf(key, value);
+		// 			var newtree := mkTwoNode(newleft, tree.key, tree);
+		// 			assert(Height(newleft) == Height(tree));
+		// 			assert(Height(newtree) == Height(tree) + 1);
+		// 			result := InsertionResult(newtree, true);
+		// 		}
+		// 	} else if tree.TwoNode? {
+		// 		if Keyspace.lt(key, tree.pivot) {
+		// 			var subresult := InsertIntoSubtree(tree.left, key, value);
+		// 			if !subresult.split {
+		// 				result := InsertionResult(mkTwoNode(subresult.tree, tree.pivot, tree.right), false);
+		// 			} else {
+		// 				result := InsertionResult(mkThreeNode(subresult.tree.left, subresult.tree.pivot,
+		// 			    subresult.tree.right, tree.pivot,
+		// 					tree.right), false);
+		// 			}
+		// 		} else {
+		// 			var subresult := InsertIntoSubtree(tree.right, key, value);
+		// 			if !subresult.split {
+		// 				result := InsertionResult(mkTwoNode(tree.left, tree.pivot, subresult.tree), false);
+		// 			} else {
+		// 				result := InsertionResult(mkThreeNode(tree.left, tree.pivot,
+		// 	        subresult.tree.left, subresult.tree.pivot,
+		// 					subresult.tree.right), false);
+		// 			}
+		// 		}
+		// 	} else if tree.ThreeNode? {
+		// 		if Keyspace.lt(key, tree.pivota) {
+		// 			var subresult := InsertIntoSubtree(tree.left, key, value);
+		// 			if !subresult.split {
+		// 				result := InsertionResult(mkThreeNode(subresult.tree, tree.pivota,
+		// 			    tree.middle, tree.pivotb,
+		// 					tree.right), false);
+		// 			} else {
+		// 				var newright := mkTwoNode(tree.middle, tree.pivotb, tree.right);
+		// 				assert(Height(newright) == Height(tree));
+		// 				var newtree := mkTwoNode(subresult.tree, tree.pivota, newright);
+		// 				assert(Height(newtree) == Height(tree) + 1);
+		// 				result := InsertionResult(newtree, true);
+		// 			}
+		// 		} else if Keyspace.lt(key, tree.pivotb) {
+		// 			var subresult := InsertIntoSubtree(tree.middle, key, value);
+		// 			if !subresult.split {
+		// 				result := InsertionResult(mkThreeNode(tree.left, tree.pivota,
+		// 			    subresult.tree, tree.pivotb,
+		// 					tree.right), false);
+		// 			} else {
+		// 				var newleft := mkTwoNode(tree.left, tree.pivota, subresult.tree.left);
+		// 				var newright := mkTwoNode(subresult.tree.right, tree.pivotb, tree.right);
+		// 				var newtree := mkTwoNode(newleft, subresult.tree.pivot, newright);
+		// 				assert(Height(newleft) == Height(tree));
+		// 				assert(Height(newright) == Height(tree));
+		// 				assert(Height(newtree) == Height(tree) + 1);
+		// 				result := InsertionResult(newtree, true);
+		// 			}
+		// 		} else {
+		// 			var subresult := InsertIntoSubtree(tree.right, key, value);
+		// 			if !subresult.split {
+		// 				result := InsertionResult(mkThreeNode(tree.left, tree.pivota,
+		// 			    tree.middle, tree.pivotb,
+		// 					subresult.tree), false);
+		// 			} else {
+		// 				var newleft := TwoNode(tree.left, tree.pivota, tree.middle);
+		// 				var newtree := TwoNode(newleft, tree.pivotb, subresult.tree);
+		// 				assert(Height(newleft) == Height(tree));
+		// 				assert(Height(newtree) == Height(tree) + 1);
+		// 				result := InsertionResult(newtree, true);
+		// 			}
+		// 		}
+		// 	} 
+		// }
+
+		// datatype Tree<Value> = EmptyTree | NonEmptyTree(root: Node<Value>)
+		
+		// predicate TTTree<Value>(tree: Tree<Value>) {
+		// 	tree.EmptyTree? || TTSubtree(tree.root)
+// }
+
+// function Contents<Value>(tree: Tree<Value>) : map<Key, Value>
+// {
+// 	if tree.EmptyTree?
+// 		then map[]
+// 	else
+// 		SubtreeContents(tree.root)
+// }
+
+// function method Query<Value>(tree: Tree<Value>, key: Key) : QueryResult<Value>
+// 	requires(TTTree(tree));
+//   ensures Query(tree, key) == KeyDoesNotExist <==>
+// 		(key !in Contents(tree));
+//   ensures Query(tree, key).ValueForKey? <==>
+// 		(key in Contents(tree) && Contents(tree)[key] == Query(tree, key).value);
+// {
+// 	if tree.EmptyTree? then
+// 		KeyDoesNotExist
+// 	else
+// 		QuerySubtree(tree.root, key)
+// }
+
+// method Insert<Value>(tree: Tree<Value>, key: Key, value: Value) returns (newtree: Tree<Value>)
+// 	requires TTTree(tree);
+// 	ensures TTTree(newtree);
+// 	ensures Contents(newtree) == Contents(tree)[key := value];
+// 	ensures newtree.NonEmptyTree?;
+// {
+// 	if tree.EmptyTree? {
+// 		newtree := NonEmptyTree(Leaf(key, value));
+// 	} else {
+// 		var result := InsertIntoSubtree(tree.root, key, value);
+// 		newtree := NonEmptyTree(result.tree);
+// 	}
+// }
 
 // datatype DeletionResult = DeletionResult(tree: Tree, merged: bool)
-	
+
 // function DeleteFromSubtree(tree: Tree, key: int) : DeletionResult
 // 	requires TTTree(tree);
 // 	ensures TTTree(result.tree);
@@ -354,9 +524,10 @@ method Insert<Value>(tree: Tree<Value>, key: int, value: Value) returns (newtree
 // 					if !subresult.merged then
 // 						DeletionResult(NonEmptyTree(subresult.root, tree.root.pivot, tree.root.right))
 // 					else
-						
+
 // 				} else {
 // 				}
 // 		}
 // }
 
+}
