lexical.dfy
@@ -1,0 +1,199 @@
+include "total_order.dfy"
+	
+module Lexically_Ordered_Strings refines Totally_Ordered_Type {
+
+ 	type Element = string
+
+	predicate method lt(a: Element, b: Element)
+		ensures lt(a, b) == ltdef(a, b);
+	{
+		if |a| == 0 && |b| == 0 then false
+		else if |a| == 0       then true
+		else if |b| == 0       then false
+		else if a[0] < b[0]    then true
+		else if a[0] > b[0]    then false
+		else lt(a[1..], b[1..])
+		// ltlte_is_transitive_forall();
+		// if |a| == 0 && |b| == 0 {
+		// 	r := false;
+		// } else if |a| == 0 {
+		// 	r := true;
+		// } else if |b| == 0 {
+		// 	r := false;
+		// } else if a[0] < b[0] {
+		// 	r := true;
+		// } else if a[0] > b[0] {
+		// 	r := false;
+		// } else {
+		// 	r := lt(a[1..], b[1..]);
+		// }
+	}
+
+	predicate method lte(a: Element, b: Element) 
+	{
+		ltedef_is_transitive_forall();
+		ltlte_is_transitive_forall();
+		ltedef_is_anti_symmetric_forall();
+		if a == b then
+			true
+		else
+			lt(a, b)
+	}
+
+	predicate ltdef(a: Element, b: Element)
+	{
+		if |a| == 0 && |b| == 0 then false
+		else if |a| == 0       then true
+		else if |b| == 0       then false
+		else if a[0] < b[0]    then true
+		else if a[0] > b[0]    then false
+		else ltdef(a[1..], b[1..])
+	}
+
+
+	predicate ltedef(a: Element, b: Element)
+	{
+		a == b || ltdef(a, b)
+	}
+
+	/////////////////////////////////////////
+	
+	lemma ltdef_is_transitive(a: string, b: string, c: string)
+		requires ltdef(a, b);
+		requires ltdef(b, c);
+		ensures ltdef(a, c);
+	{
+	}
+
+	lemma ltedef_is_transitive(a: string, b: string, c: string)
+		requires ltedef(a, b);
+		requires ltedef(b, c);
+		ensures ltedef(a, c);
+	{
+		if ltdef(a,b) && ltdef(b,c) {
+			ltdef_is_transitive(a, b, c);
+		}
+	}
+
+	lemma ltedef_is_transitive_forall()
+		ensures forall a, b, c :: ltedef(a, b) && ltedef(b, c) ==> ltedef(a, c);
+	{
+		forall a, b, c | ltedef(a, b) && ltedef(b, c) {
+			ltedef_is_transitive(a, b, c);
+		}
+	}
+
+	lemma ltlte_is_transitive(a: string, b: string, c: string)
+		requires ltdef(a, b);
+		requires ltedef(b, c);
+		ensures ltdef(a, c);
+	{
+		if ltdef(a,b) && ltdef(b,c) {
+			ltdef_is_transitive(a, b, c);
+		}
+	}
+
+	lemma ltlte_is_transitive_forall()
+		ensures forall a, b, c :: ltdef(a, b) && ltedef(b, c) ==> ltdef(a, c);
+	{
+		forall a, b, c | ltdef(a, b) && ltedef(b, c) {
+			ltlte_is_transitive(a, b, c);
+		}
+	}
+
+	lemma ltedef_is_anti_symmetric(a: string, b: string)
+		requires ltedef(a, b);
+		requires ltedef(b, a);
+		ensures a == b;
+	{
+		if |a| > 0 && |b| > 0 {
+			ltedef_is_anti_symmetric(a[1..], b[1..]);
+		}
+	}
+
+	lemma ltedef_is_anti_symmetric_forall()
+		ensures forall a, b :: ltedef(a, b) && ltedef(b, a) ==> a == b;
+	{
+		forall a, b | ltedef(a, b) && ltedef(b, a) {
+			ltedef_is_anti_symmetric(a, b);
+		}
+	}
+
+
+
+
+	
+// predicate method lte(a: string, b: string)
+	// 	ensures forall a, b, c :: lexical_lte(a, b) && lexical_lte(b, c) ==> lexical_lte(a, c);
+	// 	ensures forall a, b :: lexical_lte(a, b) && lexical_lte(b, a) ==> a == b;
+	// {
+	// 	lexical_lte_is_transitive_forall();
+	// 	lexical_lte_is_anti_symmetric_forall();
+	// 	lexical_lte(a, b)
+	// }
+
+	// function method lcp<T(==)>(a: seq<T>, b: seq<T>) : seq<T>
+	// 	ensures lcp<T>(a, b) <= a;
+	// 	ensures lcp<T>(a, b) <= b;
+	// 	ensures	|lcp<T>(a, b)| == |a| ||	|lcp<T>(a, b)| == |b| ||	a[|lcp<T>(a, b)|] != b[|lcp<T>(a, b)|];
+	// 	ensures forall a, b, c :: lte(a, b) && lte(b, c) ==>
+	// 		longest_common_prefix<char>(a, c) == longest_common_prefix<char>(a, b) ||
+	// 		longest_common_prefix<char>(a, c) == longest_common_prefix<char>(b, c);
+	// {
+	// 	longest_common_prefix(a, b)
+	// }
+	
+	// ///////////// Not revealed ///////////////////
+	
+	// predicate method lexical_lt(a: string, b: string)
+	// 	ensures lexical_lt(a, b) ==> a != b;
+	// {
+	// 	if |a| == 0 && |b| == 0 then false
+	// 	else if |a| == 0       then true
+	// 	else if |b| == 0       then false
+	// 	else if a[0] < b[0]    then true
+	// 	else if a[0] > b[0]    then false
+	// 	else lexical_lt(a[1..], b[1..])
+	// }
+
+
+	// predicate method lexical_lte(a: string, b: string)
+	// {
+	// 	a == b || lexical_lt(a, b)
+	// }
+
+
+
+	// function method longest_common_prefix<T(==)>(a: seq<T>, b: seq<T>) : seq<T>
+	// 	ensures longest_common_prefix<T>(a, b) <= a;
+	// 	ensures longest_common_prefix<T>(a, b) <= b;
+	// 	ensures
+	// 		|longest_common_prefix<T>(a, b)| == |a| ||
+	// 		|longest_common_prefix<T>(a, b)| == |b| ||
+	// 		a[|longest_common_prefix<T>(a, b)|] != b[|longest_common_prefix<T>(a, b)|];
+	// {
+	// 	if |a| == 0 || |b| == 0 || a[0] != b[0] then []
+	// 	else [a[0]] + longest_common_prefix<T>(a[1..], b[1..])
+	// }
+
+	// lemma lexical_cmp_between_implies_common_prefix(a: string, b: string, c: string)
+	// 	requires lexical_lte(a, b);
+	// 	requires lexical_lte(b, c);
+	// 	ensures
+	// 		longest_common_prefix<char>(a, c) == longest_common_prefix<char>(a, b) ||
+	// 		longest_common_prefix<char>(a, c) == longest_common_prefix<char>(b, c);
+	// {
+	// 	if |longest_common_prefix<char>(a, c)| > 0 {
+	// 		assert a[0] == b[0] && b[0] == c[0];
+	// 		lexical_cmp_between_implies_common_prefix(a[1..], b[1..], c[1..]);
+	// 	}
+	// }
+
+	// lemma lexical_cmp_between_implies_common_prefix_forall()
+	// 	ensures forall a, b, c :: lexical_lte(a, b) && lexical_lte(b, c) ==>
+	// 	longest_common_prefix<char>(a, c) == longest_common_prefix<char>(a, b) ||
+	// 	longest_common_prefix<char>(a, c) == longest_common_prefix<char>(b, c);
+	// {
+	// }
+
+}
