map_utils.dfy
@@ -1,0 +1,37 @@
+module Map_Utils {
+
+	// Requires disjoint domains and delivers predictable result.
+	function method {:opaque} disjoint_union<U,T>(mapa: map<U,T>, mapb: map<U,T>) : map<U,T>
+		requires mapa.Keys !! mapb.Keys;
+		ensures disjoint_union(mapa, mapb).Keys == mapa.Keys + mapb.Keys;
+		ensures mapa.Keys != {} || mapb.Keys != {} ==> disjoint_union(mapa, mapb).Keys != {};
+		ensures forall k :: k in mapa.Keys ==> mapa[k] == disjoint_union(mapa, mapb)[k];
+		ensures forall k :: k in mapb.Keys ==> mapb[k] == disjoint_union(mapa, mapb)[k];
+	{
+		map x : U | (x in mapa.Keys + mapb.Keys) :: if x in mapa then mapa[x] else mapb[x]
+	}
+
+	// Doesn't require disjoint domains, but guarantees to take A's
+	// definition.
+	function method {:opaque} union_preferA<U,T>(mapa: map<U,T>, mapb: map<U,T>) : map<U,T>
+		ensures union_preferA(mapa, mapb).Keys == mapa.Keys + mapb.Keys;
+		ensures mapa.Keys != {} || mapb.Keys != {} ==> union_preferA(mapa, mapb).Keys != {};
+		ensures forall k :: k in mapa.Keys ==> mapa[k] == union_preferA(mapa, mapb)[k];
+		ensures forall k :: k in mapb.Keys - mapa.Keys ==> mapb[k] == union_preferA(mapa, mapb)[k];
+	{
+		map x : U | (x in mapa.Keys + mapb.Keys) :: if x in mapa then mapa[x] else mapb[x]
+	}
+
+	// Doesn't require disjoint domains, and makes no promises about
+	// which it chooses on the intersection.
+	function method {:opaque} union<U,T>(mapa: map<U,T>, mapb: map<U,T>) : map<U,T>
+		ensures union(mapa, mapb).Keys == mapa.Keys + mapb.Keys;
+		ensures mapa.Keys != {} || mapb.Keys != {} ==> union(mapa, mapb).Keys != {};
+		ensures forall k :: k in mapa.Keys -mapb.Keys ==> mapa[k] == union(mapa, mapb)[k];
+		ensures forall k :: k in mapb.Keys - mapa.Keys ==> mapb[k] == union(mapa, mapb)[k];
+		ensures forall k :: k in mapa.Keys * mapb.Keys ==>
+			mapb[k] == union(mapa, mapb)[k] || mapa[k] == union(mapa, mapb)[k];
+	{
+		union_preferA(mapa, mapb)
+	}
+}
