total_order.dfy
@@ -1,0 +1,22 @@
+abstract module Totally_Ordered_Type {
+
+	type Element(!new,==)
+
+	predicate method lt(a: Element, b: Element)
+		ensures lt(a, b) == ltdef(a, b);
+		ensures ltdef(a, b) || ltdef(b, a) || a == b; 
+		ensures ltdef(a, b) ==> a != b && !ltdef(b, a); 
+		ensures forall a, b, c :: ltdef(a, b) && ltdef(b, c) ==> ltdef(a, c);
+		// ensures forall a, b, c :: ltdef(a, b) && ltedef(b, c) ==> ltdef(a, c);
+		// ensures forall a, b, c :: ltedef(a, b) && ltdef(b, c) ==> ltdef(a, c);
+
+	// predicate method lte(a: Element, b: Element)
+	// 	ensures lte(a, b) == ltedef(a, b);
+	// 	ensures forall a, b :: ltedef(a, b) && ltedef(b, a) ==> a == b;
+	// 	ensures forall a, b, c :: ltedef(a, b) && ltedef(b, c) ==> ltedef(a, c);
+		// ensures forall a, b, c :: ltdef(a, b) && ltedef(b, c) ==> ltdef(a, c);
+		// ensures forall a, b, c :: ltedef(a, b) && ltdef(b, c) ==> ltdef(a, c);
+		
+	predicate ltdef(a: Element, b: Element)
+	//predicate ltedef(a: Element, b: Element)
+}
